coqimp/framework/soundness/wfcdhp_sound.v
@@ -6,17 +6,17 @@ Require Import Integers.
 Open Scope Z_scope.  
 Import ListNotations.
 
-Set Asymmetric Patterns.
-   
+Set Asymmetric Patterns. 
+    
 Require Import state. 
 Require Import language.
 
-Set Implicit Arguments.
+Set Implicit Arguments. 
 Unset Strict Implicit.
-         
+           
 Require Import logic. 
 Require Import soundness.
- 
+  
 Require Import lemmas.
 
 Require Import inssound.
@@ -25,6 +25,1146 @@ Require Import Coq.Logic.FunctionalExtensionality.
  
 Open Scope nat.
 Open Scope code_scope.
+
+(*+ trivial Lemma +*) 
+Lemma sep_reg_dec :
+  forall (s s' : SpReg),
+    {s = s'} + {s <> s'}.
+Proof.
+  intros.
+  destruct s; destruct s'; eauto;
+    try solve [right; intro; tryfalse].
+  destruct a; destruct a0; eauto;
+    try solve [right; intro; tryfalse].
+Qed.
+
+(*+ Lemmas for register state +*)
+Lemma indom_setR_eq_RegMap_set :
+  forall (s : RegName) R w,
+    indom s R ->
+    set_R R s w = RegMap.set s (Some w) R.
+Proof.
+  intros.
+  unfold set_R.
+  unfold is_indom.
+  destruct (R s) eqn:Heqe; eauto.
+  unfold indom in H.
+  simpljoin1.
+  rewrite H in Heqe.
+  tryfalse.
+Qed.
+
+Lemma regset_l_l_indom :
+  forall rn v m,
+    indom rn (RegMap.set rn (Some v) m).
+Proof.
+  intros.
+  unfold indom.
+  exists v.
+  unfolds RegMap.set.
+  destruct_rneq.
+Qed.
+
+Lemma regset_twice :
+  forall (A : Type) l (v v1 : A) m,
+    RegMap.set l (Some v) (RegMap.set l (Some v1) m) =
+    RegMap.set l (Some v) m.
+Proof.
+  intros.
+  eapply functional_extensionality.
+  intro.
+  unfolds RegMap.set.
+  destruct_rneq.
+Qed.
+  
+(*+ Lemmas for delay list +*)
+Lemma not_in_exe_dly_stable :
+  forall D R R' D' s,
+    exe_delay R D = (R', D') ->
+    ~ In s (getRegs D) ->
+    ~ In s (getRegs D').
+Proof.
+  intro D.
+  induction D; intros.
+  -
+    simpl in H.
+    inversion H; subst.
+    intro.
+    simpls.
+    tryfalse.
+  -
+    destruct a, p.
+    simpl in H.
+    destruct d.
+    {
+      destruct (exe_delay R D) eqn:Heqe1; eauto.
+      inversion H; subst.
+      eapply IHD in Heqe1; eauto.
+      intro.
+      eapply H0.
+      simpl.
+      eauto.
+    }
+    {
+      destruct (exe_delay R D) eqn:Heqe1; eauto.
+      inversion H; subst.
+      eapply IHD with (s := s) in Heqe1; eauto.
+      intro.
+      simpl in H1.
+      destruct H1; subst.
+      eapply H0.
+      simpl; eauto.
+      eapply Heqe1; eauto.
+      intro.
+      eapply H0.
+      simpl; eauto.
+    }
+Qed.
+
+Lemma dlyitem_in_dlyls_reg_in :
+  forall D t s w,
+    In (t, s, w) D ->
+    In s (getRegs D).
+Proof.
+  intro D.
+  induction D; intros.
+  -
+    simpls; eauto.
+  -
+    destruct a, p.
+    simpl in H.
+    destruct H.
+    inversion H; subst.
+    simpl; eauto.
+    simpl.
+    right.
+    eauto.
+Qed.
+
+Lemma dlytime_gt_zero_exe_still :
+  forall D t s w D' R R',
+    In (S t, s, w) D -> (R', D') = exe_delay R D ->
+    In (t, s, w) D'.
+Proof.
+  intro D.
+  induction D; intros.
+  -
+    simpl in H0.
+    inversion H0; subst.
+    simpl in H.
+    tryfalse.
+  -
+    destruct a, p.
+    simpl in H.
+    destruct H.
+    {
+      inversion H; subst.
+      simpl in H0. 
+      destruct (exe_delay R D) eqn:Heqe; eauto.
+      inversion H0; subst.
+      simpl; eauto.
+    }
+    {
+      simpl in H0.
+      destruct n.
+      {
+        destruct (exe_delay R D) eqn:Heqe; eauto.
+        inversion H0; subst.
+        symmetry in Heqe.
+        eapply IHD in Heqe; eauto.
+      }
+      {
+        destruct (exe_delay R D) eqn:Heqe; eauto.
+        inversion H0; subst.
+        symmetry in Heqe.
+        eapply IHD in Heqe; eauto.
+        simpl; eauto.
+      }
+    }
+Qed.
+    
+Lemma noDup_exe_dly_stable :
+  forall D R R' D',
+    noDup (getRegs D) ->
+    exe_delay R D = (R', D') ->
+    noDup (getRegs D').
+Proof.
+  intro D.
+  induction D; intros.
+  -
+    simpl in H0.
+    inversion H0; subst.
+    econstructor; eauto.
+  -
+    destruct a, p.
+    simpl in H0.
+    destruct d.
+    {
+      destruct (exe_delay R D) eqn:Heqe.
+      inversion H0; subst.
+      simpl in H.
+      inversion H; subst.
+      eauto.
+    }
+    {
+      destruct (exe_delay R D) eqn:Heqe.
+      inversion H0; subst.
+      simpl in H.
+      inversion H; subst.
+      simpl.
+      econstructor; eauto.
+      eapply not_in_exe_dly_stable; eauto.
+    }
+Qed.
+
+Lemma regdlySt_dly_nil_false :
+  forall n s w M R F,
+    regdlySt n s w (M, (R, F), []) -> False.
+Proof.
+  intro n.
+  induction n; intros.
+  -
+    simpls.
+    unfolds inDlyBuff.
+    simpljoin1.
+    simpls; tryfalse.
+  -
+    simpl in H.
+    destruct H.
+    unfolds inDlyBuff.
+    simpljoin1.
+    simpls.
+    tryfalse.
+    eauto.
+Qed.
+
+Lemma regdlySt_dlyls_relevent :
+  forall t D s w M M' R R' F F',
+    regdlySt t s w (M, (R, F), D) ->
+    regdlySt t s w (M', (R', F'), D).
+Proof.
+  intro t.
+  induction t; intros.
+  -
+    unfolds regdlySt.
+    simpls.
+    eauto.
+  -
+    simpls.
+    destruct H; eauto.
+Qed.
+    
+Lemma dly_reduce_Aemp_stable :
+  forall D M R R' F D',
+    (M, (R, F), D) |= Aemp -> (R', D') = exe_delay R D ->
+    (M, (R', F), D') |= Aemp.
+Proof.
+  intros D.
+  induction D; intros.
+  -
+    simpls.
+    inversion H0; eauto.
+  -
+    destruct a, p.
+    assert ((M, (R, F), D) |= Aemp).
+    {
+      clear - H.
+      simpls; eauto.
+    }
+
+    simpl in H0.
+    destruct d.
+    {
+      destruct (exe_delay R D) eqn:Heqe; eauto.
+      inversion H0; subst.
+      eapply IHD with (R' := r) (D' := d) in H1; eauto.
+      simpl in H.
+      simpljoin1.
+      simpls.
+      simpljoin1.
+      split; eauto.
+    }
+    {
+      destruct (exe_delay R D) eqn:Heqe; eauto.
+      inversion H0; subst.
+      eapply IHD with (R' := r) (D' := d0) in H1; eauto.
+    }
+Qed.
+
+Lemma dly_reduce_Amapsto_stable :
+  forall D M R R' F D' a w,
+    (M, (R, F), D) |= a |-> w -> (R', D') = exe_delay R D ->
+    (M, (R', F), D') |= a |-> w.
+Proof.
+  intros D.
+  induction D; intros.
+  -
+    simpls.
+    inversion H0; eauto.
+  -
+    destruct a, p.
+    assert ((M, (R, F), D) |= a0 |-> w).
+    {
+      clear - H.
+      simpls.
+      eauto.
+    }
+
+    simpl in H0.
+    destruct d.
+    {
+      destruct (exe_delay R D) eqn:Heqe.
+      inversion H0; subst.
+      eapply IHD with (R' := r) (D' := d) in H1; eauto.
+      simpls.
+      simpljoin1; eauto.
+    }
+    {
+      destruct (exe_delay R D) eqn:Heqe.
+      inversion H0; subst.
+      eapply IHD with (R' := r) (D' := d0) in H1; eauto.
+    }
+Qed.
+
+Lemma dly_reduce_Aaexp_stable :
+  forall D M R R' F D' a a0,
+    (M, (R, F), D) |= a ==ₓ a0 -> (R', D') = exe_delay R D ->
+    (M, (R', F), D') |= a ==ₓ a0.
+Proof.
+  intros D.
+  induction D; intros.
+  -
+    simpls.
+    simpljoin1.
+    eauto.
+  -
+    destruct a, p.
+    assert ((M, (R, F), D) |= a0 ==ₓ a1).
+    {
+      clear - H.
+      simpls.
+      eauto.
+    }
+
+    simpl in H0.
+    destruct d.
+    {
+      destruct (exe_delay R D) eqn:Heqe.
+      inversion H0; subst.   
+      eapply IHD with (R' := r) (D' := d) in H1; eauto.
+      clear - H1.
+      simpls.
+      simpljoin1.
+      unfolds eval_addrexp.
+      destruct a0; eauto.
+      split; eauto.
+
+      unfolds eval_opexp.
+      destruct o; eauto.
+      unfold set_R.
+      unfold is_indom.
+      destruct (r s) eqn :Heqe; eauto.
+      unfolds RegMap.set.
+      destruct_rneq; eauto.
+      unfold set_R.
+      unfold is_indom.
+      destruct (r s) eqn:Heqe; eauto.
+      unfold RegMap.set.
+      destruct_rneq; eauto.
+      destruct (r g) eqn:Heqe2; eauto.
+      unfolds eval_opexp.
+      destruct o; eauto.
+      destruct_rneq; eauto.
+    }
+    {
+      destruct (exe_delay R D) eqn:Heqe; subst.
+      inversion H0; subst.
+      eapply IHD with (R' := r) (D' := d0) in H1; eauto.
+    }
+Qed.
+
+Lemma dly_reduce_Aoexp_stable :
+  forall D M R R' F D' o w,
+    (M, (R, F), D) |= o ==ₑ w -> (R', D') = exe_delay R D ->
+    (M, (R', F), D') |= o ==ₑ w.
+Proof.
+  intros D.
+  induction D; intros.
+  -
+    simpl in H0.
+    inversion H0; eauto.
+  -
+    destruct a, p.
+    assert ((M, (R, F), D) |= o ==ₑ w).
+    {
+      clear - H.
+      simpls.
+      eauto.
+    }
+
+    simpl in H0.
+    destruct d.
+    {
+      destruct (exe_delay R D) eqn:Heqe; eauto.
+      inversion H0; subst.
+      eapply IHD with (R' := r) (D' := d) in H1; eauto.
+      clear - H1.
+      simpls.
+      unfolds eval_opexp.
+      destruct o; eauto.
+      unfolds set_R.
+      unfold is_indom.
+      destruct (r s); eauto.
+      unfolds RegMap.set.
+      destruct_rneq; eauto.
+    }
+    {
+      destruct (exe_delay R D) eqn:Heqe; eauto.
+      inversion H0; subst.
+      eapply IHD with (R' := r) (D' := d0) in H1; eauto.
+    }
+Qed.
+
+Lemma dly_reduce_reg_stable :
+  forall D M R R' F D' r w,
+    (M, (R, F), D) |= r |=> w -> (R', D') = exe_delay R D ->
+    (M, (R', F), D') |= r |=> w.
+Proof.
+  intro D.
+  induction D; intros.
+  -
+    simpls.
+    inversion H0; eauto.
+  -
+    destruct a, p.
+    assert ((M, (R, F), D) |= r |=> w).
+    {
+      clear - H.
+      simpls.
+      unfolds regSt.
+      simpljoin1; eauto.
+      simpls.
+      repeat (split; eauto).
+      intro.
+      eapply H1.
+      clear - H2.
+      unfolds regInDlyBuff.
+      destruct r; eauto; tryfalse.
+      simpls.
+      eauto.
+    }
+
+    simpl in H0.
+    destruct d.
+    {
+      destruct (exe_delay R D) eqn:Heqe.
+      inversion H0; subst. 
+      eapply IHD with (R' := r0) (D' := d) in H1; eauto.
+      clear - H1 H.
+      simpls.
+      unfolds regSt.
+      simpls.
+      simpljoin1.
+      repeat (split; eauto).
+      unfold set_R.
+      unfold is_indom.
+      unfold RegMap.set.
+      destruct_rneq.
+      subst.
+      false.
+      eapply H4.
+      unfold regInDlyBuff.
+      simpl; eauto.
+    }
+    {
+      destruct (exe_delay R D) eqn:Heqe.
+      inversion H0; subst.
+      eapply IHD with (R' := r0) (D' := d0) in H1; eauto.
+      clear - H H1.
+      simpls.
+      unfolds regSt.
+      simpls.
+      simpljoin1; eauto.
+      repeat (split; eauto).
+      intro. 
+      eapply H2.
+      clear - H H4.
+      unfolds regInDlyBuff.
+      destruct r; eauto; tryfalse.
+      simpls; eauto.
+      destruct H; eauto.
+      subst.
+      false.
+      eapply H4; eauto.
+    }
+Qed.
+
+Lemma reg_not_in_dlybuff_exe_dly_stable :
+  forall D D' R' (s : SpReg) v,
+    exe_delay (RegMap.set s (Some v) empR) D = (R', D') ->
+    ~ In s (getRegs D) ->
+    R' = RegMap.set s (Some v) empR.
+Proof.
+  intro D.
+  induction D; intros.
+  -
+    simpl in H.
+    inversion H; eauto.
+  -
+    destruct a, p.
+    simpl in H0.
+    simpl in H.
+    destruct d.
+    {
+      destruct (exe_delay (RegMap.set s (Some v) empR) D) eqn:Heqe.
+      inversion H; subst.
+      eapply IHD in Heqe; eauto.
+      subst.
+ 
+      unfold set_R.
+      unfold is_indom.
+      unfold RegMap.set.
+      destruct (sep_reg_dec s0 s); tryfalse.
+      {
+        false.
+        eapply H0; eauto.
+      }
+      {
+        destruct_rneq.
+      }
+    }
+    {
+      destruct (exe_delay (RegMap.set s (Some v) empR) D) eqn:Heqe; eauto.
+      inversion H; subst.
+      eapply IHD in Heqe; eauto.
+    }
+Qed.
+    
+Lemma dlytime_zero_exe_dly :
+  forall D M R R' F D' s w,
+    (M, (R, F), D) |= 0 @ s |==> w ->
+    (R', D') = exe_delay R D ->
+    (M, (R', F), D') |= s |=> w.
+Proof.
+  intro D.
+  induction D; intros.
+  -
+    simpl in H.
+    simpljoin1.
+    destruct H2.
+    {
+      unfolds inDlyBuff.
+      simpljoin1.
+      simpl in H.
+      tryfalse.
+    }
+    {
+      simpl in H0.
+      inversion H0; subst.
+      unfolds regSt.
+      simpls.
+      simpljoin1.
+      eapply equal_f in H.
+      assert (RegMap.set s (Some x) empR s = RegMap.set s (Some w) empR s); eauto.
+      clear - H.
+      unfold RegMap.set in H.
+      destruct_rneq_H.
+      inversion H; subst.
+      unfold regSt.
+      simpl; eauto.
+    }
+  - 
+    destruct a, p.
+    simpl in H0. 
+    destruct d.
+    {
+      destruct (exe_delay R D) eqn:Heqe.
+      inversion H0; subst.
+
+      lets Ht : H.
+      simpl in Ht.
+      simpljoin1.
+      destruct H3.
+      {
+        unfolds inDlyBuff.
+        simpljoin1.
+        simpl in H0.
+        destruct H0.
+        { 
+          inversion H0; subst.
+          simpl in H1.
+          inversion H1; subst.
+          lets Hexe_dly : Heqe.
+          eapply reg_not_in_dlybuff_exe_dly_stable in Heqe; eauto.
+          subst.
+          simpl.
+          unfold regSt.
+          simpl.
+          repeat (split; eauto).
+          rewrite indom_setR_eq_RegMap_set; eauto.
+          rewrite regset_twice; eauto.
+          eapply regset_l_l_indom; eauto.
+          eapply not_in_exe_dly_stable; eauto.
+        }
+        {
+          inversion H1; subst.
+          assert (s <> s0).
+          {
+            intro.
+            subst.
+            eapply dlyitem_in_dlyls_reg_in in H0; eauto.
+          }
+
+          assert ((empM, (RegMap.set s (Some x) empR, F), D) |= 0 @ s |==> w).
+          {
+            clear - H H2.
+            simpls.
+            simpljoin1.
+            destruct H1.
+            unfold inDlyBuff in H0.
+            simpljoin1.
+            simpl in H0.
+            destruct H0.
+            inversion H0; subst; tryfalse.
+            exists x.
+            repeat (split; eauto).
+            left.
+            unfold inDlyBuff.
+            simpl in H1.
+            inversion H1; eauto.
+            exists x.
+            repeat (split; eauto).
+            right.
+            unfolds regSt.
+            simpls.
+            simpljoin1; eauto.
+            repeat (split; eauto).
+          }
+
+          eapply IHD with (R' := r) (D' := d) in H3; eauto.
+          clear - H2 H3.
+          simpls.
+          unfolds regSt.
+          simpls.
+          simpljoin1.
+          repeat (split; eauto).
+          unfold set_R.
+          unfold is_indom.
+          unfold RegMap.set at 1.
+          destruct_rneq.
+        }
+      }
+      {
+        assert ((empM, (RegMap.set s (Some x) empR, F), D) |= 0 @ s |==> w).
+        { 
+          clear - H0.
+          simpl.
+          exists x.
+          repeat (split; eauto).
+          right.
+          unfolds regSt.
+          simpls.
+          simpljoin1.
+          repeat (split; eauto).
+        }
+
+        eapply IHD with (R' := r) (D' := d) in H1; eauto.
+
+        assert (s <> s0).
+        {
+          clear - H0.
+          unfolds regSt.
+          simpls.
+          simpljoin1.
+          intro.
+          eapply H1; eauto.
+        }
+
+        clear - H1 H2.
+        simpls.
+        unfolds regSt.
+        simpls.
+        simpljoin1.
+        repeat (split; eauto).
+        unfold set_R.
+        unfold is_indom.
+        unfold RegMap.set.
+        destruct_rneq.
+      }
+    }
+    {
+      destruct (exe_delay R D) eqn:Heqe.
+      inversion H0; subst.
+
+      assert ((M, (R, F), D) |= 0 @ s |==> w).
+      {
+        clear - H.
+        simpls.
+        simpljoin1.
+        exists x.
+        repeat (split; eauto).
+        destruct H1.
+        {
+          unfolds inDlyBuff.
+          simpljoin1.
+          simpl in H.
+          destruct H.
+          inversion H.
+          inversion H0; subst; eauto.
+        }
+        {
+          right.
+          unfolds regSt.
+          simpls.
+          simpljoin1.
+          repeat (split; eauto).
+        }
+      }
+
+      eapply IHD with (R' := r) (D' := d0) in H1; eauto.
+
+      assert (s <> s0).
+      { 
+        clear - H.
+        intro.
+        subst.
+        simpls.
+        simpljoin1.
+        destruct H1.
+        unfolds inDlyBuff.
+        simpls; simpljoin1.
+        destruct H.
+        inversion H; tryfalse.
+        inversion H0; subst.
+        eapply dlyitem_in_dlyls_reg_in in H; eauto.
+        unfolds regSt.
+        simpls.
+        simpljoin1.
+        eauto.
+      }
+
+      clear - H1 H2.
+      simpls.
+      unfolds regSt.
+      simpls.
+      simpljoin1.
+      repeat (split; eauto).
+      intro.
+      destruct H; tryfalse.
+    }
+Qed.
+
+Lemma regst_conseq_regdly :
+  forall M R F D t (s : SpReg) w,
+    (M, (R, F), D) |= s |=> w ->
+    (M, (R, F), D) |= t @ s |==> w.
+Proof.
+  intros.
+  simpls.
+  unfolds regSt.
+  simpls.
+  simpljoin1.
+  exists w.
+  repeat (split; eauto).
+Qed.
+
+Lemma regdlySt_dlycons_stable :
+  forall t t0 s s0 w w0 M R F D,
+    regdlySt t s w (M, (R, F), D) -> ~ In s0 (getRegs D) ->
+    regdlySt t s w (M, (R, F), (t0, s0, w0) :: D).
+Proof.
+  intro t.
+  induction t; intros.
+  -
+    simpls.
+    unfolds inDlyBuff.
+    simpls.
+    simpljoin1.
+    split; eauto.
+    econstructor; eauto.
+  -
+    simpls.
+    destruct H.
+    {
+      left.
+      unfolds inDlyBuff.
+      simpljoin1.
+      simpl; eauto.
+      split; eauto.
+      econstructor; eauto.
+    }
+    {
+      right.
+      eauto.
+    }
+Qed.
+
+Lemma dlytm_gt_zero_exe_dly :
+  forall D R' D' F x t (s : SpReg) w,
+    (R', D') = exe_delay (RegMap.set s (Some x) empR) D ->
+    inDlyBuff (S t, s, w) D ->
+    (empM, (R', F), D') |= t @ s |==> w.
+Proof.
+  intro D.
+  induction D; intros.
+  -
+    unfolds inDlyBuff.
+    simpls.
+    simpljoin1; tryfalse.
+  -
+    destruct a, p.
+    unfold inDlyBuff in H0.
+    simpljoin1.
+    simpl in H0. 
+    destruct H0.
+    {
+      inversion H0; subst.
+      simpl in H1.
+      simpl in H.
+      destruct (exe_delay (RegMap.set s (Some x) empR) D) eqn:Heqe.
+      inversion H; subst.
+      inversion H1; subst.
+      lets Ht : Heqe.
+      eapply reg_not_in_dlybuff_exe_dly_stable in Heqe; eauto.
+      subst.
+      simpl.
+      exists x.
+      repeat (split; eauto).
+      left.
+      destruct t; simpl; eauto.
+      unfold inDlyBuff.
+      simpl; eauto.
+      split; eauto.
+      econstructor; eauto.
+      eapply not_in_exe_dly_stable; eauto.
+      eapply noDup_exe_dly_stable; eauto.
+
+      left.
+      unfold inDlyBuff.
+      split; simpl; eauto.
+      econstructor; eauto.
+      eapply not_in_exe_dly_stable; eauto.
+      eapply noDup_exe_dly_stable; eauto.
+    }
+    {
+      simpl in H.
+      destruct d.
+      {  
+        destruct (exe_delay (RegMap.set s (Some x) empR) D) eqn:Heqe.
+        inversion H; subst.
+        symmetry in Heqe.
+        lets Ht : Heqe.
+        eapply IHD with (t := t) (w := w) (F := F) in Heqe; eauto.
+        Focus 2.
+        unfold inDlyBuff.
+        simpl in H1.
+        inversion H1; subst; eauto.
+        eapply dlytime_gt_zero_exe_still in Ht; eauto.
+        clear - Heqe Ht.
+        simpl in Heqe.
+        simpljoin1.
+        destruct H1.
+        {
+          simpl.
+          destruct (sep_reg_dec s s0).
+          {
+            subst.
+            exists w0.
+            repeat (split; eauto).
+            unfold set_R.
+            unfold is_indom.
+            unfolds RegMap.set.
+            destruct_rneq.
+            eapply functional_extensionality; eauto.
+            intros.
+            destruct_rneq.
+            left.
+            eapply regdlySt_dlyls_relevent; eauto.
+          }
+          {
+            exists x.
+            repeat (split; eauto).
+            unfold set_R.
+            unfold is_indom.
+            unfold RegMap.set.
+            destruct_rneq.
+            left.
+            eapply regdlySt_dlyls_relevent; eauto.
+          }
+        }
+        
+        unfolds regSt.
+        simpls.
+        simpljoin1.
+        eapply dlyitem_in_dlyls_reg_in in Ht; eauto.
+        tryfalse.
+      }
+      {
+        destruct (exe_delay (RegMap.set s (Some x) empR) D) eqn:Heqe.
+        inversion H; subst.
+        symmetry in Heqe.
+
+        assert (s <> s0).
+        {
+          clear - H0 H1.
+          intro.
+          subst.
+          simpl in H1.
+          inversion H1; subst.
+          eapply dlyitem_in_dlyls_reg_in in H0; eauto.
+        }
+
+        lets Ht : Heqe. 
+        eapply IHD with (t := t) (w := w) (F := F) in Heqe; eauto.
+        Focus 2. 
+        clear - H0 H1.
+        unfold inDlyBuff.
+        simpl in H1.
+        inversion H1; eauto.
+
+        simpl in H1. 
+        inversion H1; subst. 
+        clear - Heqe H2 H5 Ht.
+        simpls.
+        simpljoin1.
+        exists x0.
+        repeat (split; eauto).
+        destruct H1.
+        left.
+        eapply regdlySt_dlycons_stable; eauto.
+        eapply not_in_exe_dly_stable; eauto.
+        right.
+        clear - H H2.
+        unfolds regSt.
+        simpls.
+        simpljoin1.
+        repeat (split; eauto).
+        intro.
+        destruct H0; subst; tryfalse.
+      }
+    }
+Qed.
+
+Lemma regdlySt_in_vl_eq :
+  forall t s0 w w0 M R F D,
+    regdlySt t s0 w (M, (R, F), (0, s0, w0) :: D) ->
+    w = w0.
+Proof.
+  intro t.
+  induction t; intros.
+  -
+    simpl in H.
+    unfolds inDlyBuff.
+    simpljoin1.
+    simpl in H.
+    destruct H.
+    inversion H; eauto.
+    simpl in H0.
+    inversion H0; subst.
+    eapply dlyitem_in_dlyls_reg_in in H; eauto.
+    tryfalse.
+  - 
+    simpl in H.
+    destruct H.
+    {
+      unfolds inDlyBuff.
+      simpljoin1.
+      simpl in H.
+      destruct H.
+      inversion H; tryfalse.
+      simpl in H0.
+      inversion H0; subst.
+      eapply dlyitem_in_dlyls_reg_in in H; eauto.
+      tryfalse.
+    }
+    {
+      eauto.
+    }
+Qed.
+    
+Lemma inregdly_exe_dly_stable :
+  forall D R' D' F t (s : SpReg) w x,
+    (R', D') = exe_delay (RegMap.set s (Some x) empR) D ->
+    regdlySt t s w (empM, (RegMap.set s (Some x) empR, F), D) ->
+    (empM, (R', F), D') |= t @ s |==> w.
+Proof.
+  intro D.
+  induction D; intros.
+  -
+    simpl in H.
+    simpl in H.
+    simpls.
+    inversion H; subst.
+    exists x.
+    repeat (split; eauto).
+  -   
+    destruct a, p.
+    simpl in H.
+    destruct d.
+    {
+      destruct (exe_delay (RegMap.set s (Some x) empR) D) eqn:Heqe; eauto.
+      inversion H; subst.
+      symmetry in Heqe. 
+      destruct (sep_reg_dec s s0) eqn:Heqe1.
+      {
+        subst.
+        lets Ht : H0.
+        eapply regdlySt_in_vl_eq in H0; eauto.
+        subst.
+        simpl.
+        exists w0.
+        repeat (split; eauto).
+        symmetry in Heqe.
+        eapply reg_not_in_dlybuff_exe_dly_stable in Heqe; eauto.
+        subst.
+        rewrite indom_setR_eq_RegMap_set; eauto.
+        rewrite regset_twice; eauto.
+        eapply regset_l_l_indom; eauto.
+      }
+      
+    }
+Admitted.
+    
+Lemma dlytime_gt_zero_reduce_exe_dly :
+  forall D M R R' D' F t s w,
+    (M, (R, F), D) |= S t @ s |==> w ->
+    (R', D') = exe_delay R D ->
+    (M, (R', F), D') |= t @ s |==> w.
+Proof.
+  intros.
+  lets Ht : H.
+  simpl in Ht.
+  simpljoin1.
+
+  destruct H3.
+  { 
+    destruct H1.
+    {
+      eapply dlytm_gt_zero_exe_dly; eauto.
+    }
+    {
+    }
+  }
+  {
+    assert ((empM, (RegMap.set s (Some x) empR, F), D) |= s |=> w).
+    {
+      simpl.
+      eauto.
+    }
+
+    eapply dly_reduce_reg_stable in H2; eauto.
+    eapply regst_conseq_regdly; eauto.
+  }
+  
+Lemma dly_reduce_dlyreg_stable :
+  forall D M R R' F D' s w n,
+    (M, (R, F), D) |= n @ s |==> w ->
+    (R', D') = exe_delay R D ->
+    (M, (R', F), D') |= (n @ s |==> w ↓).
+Proof.
+  intros.
+  destruct n.
+  { 
+    simpl TimReduce.
+    eapply dlytime_zero_exe_dly; eauto.
+  }
+  {
+    simpl TimReduce.
+    
+  }
+  
+Lemma dly_reduce_asrt_stable :
+  forall p M R R' F D D',
+    (M, (R, F), D) |= p -> (R', D') = exe_delay R D ->
+    (M, (R', F), D') |= (p ↓).
+Proof.
+  intros p.
+  induction p; intros.
+
+  - (* Aemp *)
+    simpl TimReduce. 
+    eapply dly_reduce_Aemp_stable; eauto.
+
+  - (* Amapsto *)
+    simpl TimReduce.
+    eapply dly_reduce_Amapsto_stable; eauto.
+  
+  - (* Aaexp *)
+    simpl TimReduce.
+    eapply dly_reduce_Aaexp_stable; eauto.
+
+  - (* Aoexp *)
+    simpl TimReduce.
+    eapply dly_reduce_Aoexp_stable; eauto.
+
+  - (* regst *)
+    simpl TimReduce.
+    eapply dly_reduce_reg_stable; eauto.
+
+  - (* dlyregst *)
+
+   
+
+  - (* APure *)
+    simpl TimReduce.
+    simpls; eauto.
+
+  - (* AframeList *)
+    admit.
+
+  - (* Atrue *)
+    simpl TimReduce.
+    simpls; eauto.
+
+  - (* Afalse *)
+    simpl TimReduce.
+    simpls; eauto.
+
+  - (* Aconj *)
+    simpl TimReduce.
+    simpl in H. simpl.
+    simpljoin1; eauto.
+
+  - (* Adisj *)
+    simpl TimReduce.
+    simpl in H. simpl.
+    destruct H; eauto.
+
+  - (* Astar *)
+    admit.
+
+  - (* Aforall *)
+    simpl in H0.
+    simpl.
+    intros.
+    specialize (H0 x).
+    eauto.
+
+  - (* Aexists *)
+    simpl in H0.
+    simpljoin1.
+    simpl.
+    exists x.
+    eauto.
+
+(*+ Well-formed CodeHeap Proof +*)
+
+Definition ins_sound_partial (p q : asrt) (i : ins) :=
+  forall s s', s |= p -> (Q__ s (cntrans i) s') -> s' |= q.
+
+Lemma total_to_partial :
+  forall p q i,
+    ins_sound p q i -> ins_sound_partial p q i.
+Proof.
+  intros.
+  unfolds ins_sound, ins_sound_partial.
+  intros.
+  eapply H in H0; eauto.
+  simpljoin1.
+  eapply ins_exec_deterministic in H0; eauto.
+  subst.
+  eauto.
+Qed.
 
 Ltac get_ins_diff_false :=
   match goal with
@@ -39,22 +1179,27 @@ Lemma insSeq_rule_sound :
     wf_cdhp Spec C Spec' -> cdhp_subst Spec Spec' -> S |= p ->
     safety C S pc npc q 0.
 Proof.
-  cofix.
-
   intros.
-  eapply safety_cons.
+  generalize dependent pc.
+  generalize dependent npc.
+  generalize dependent S.
+  generalize dependent C.
+
+  induction H; intros.
 
   - (** Seq *)
+    inversion H4; subst.
+    eapply safety_cons;
+      try solve [intros; get_ins_diff_false].
     intros.
-    inversion H0; subst; get_ins_diff_false.
-    inversion H; subst.
-    {
-      (* Normal *)
-      inversion H5; subst.
-      inversion H18; get_ins_diff_false.
-      clear H18.
-      eapply ins_rule_sound in H14; eauto.
-    }
+
+    inversion H6; subst.
+    inversion H17; get_ins_diff_false.
+    rewrite H10 in H5; inversion H5; subst.
+    eapply ins_rule_sound in H.
+    eapply total_to_partial in H.
+
+    >>>>>>>>>>>>>>>>
     
   
 Theorem cdhp_rule_sound :
